fork from here to update the driver.ml in driver folder

compiler_test/funptr.c
@@ -1,0 +1,16 @@
+#include <stdio.h>
+
+void fun(int a) {
+  printf("Value of a is %d\n", a);
+}
+
+int main() {
+  
+    // fun_ptr is a pointer to function fun()
+    void (*fun_ptr)(int) = &fun;
+	fun(15);
+    // Invoking fun() using fun_ptr
+    (*fun_ptr)(10);
+
+    return 0;
+}
